wip

code/bignum/Hacl.Bignum.MontArithmetic.fst
@@ -28,8 +28,10 @@ friend Hacl.Spec.Bignum.MontArithmetic
 
 #set-options "--z3rlimit 50 --fuel 0 --ifuel 0"
 
-let bn_field_get_len #t k _ =
-  k.len
+let bn_field_get_len #t k =
+  let open LowStar.BufferOps in
+  let k1 = !*k in
+  k1.len
 
 
 let bn_field_check_modulus #t km n =
@@ -50,115 +52,129 @@ let bn_field_init #t km r n =
   let r2 : lbignum t len = r2 in
   let n1 : lbignum t len = n1 in
 
-  if bn_field_check_modulus km n then begin
-    copy n1 n;
+  copy n1 n;
+  let nBits = size (bits t) *! BB.unsafe_size_from_limb (BL.bn_get_top_index len n) in
+  km.BM.precomp nBits n r2;
 
-    let nBits = size (bits t) *! BB.unsafe_size_from_limb (BL.bn_get_top_index len n) in
-    km.BM.precomp nBits n r2;
-
-    let mu = BM.mod_inv_limb n.(0ul) in
-    let res : bn_mont_ctx t = { len = len; n = n1; mu = mu; r2 = r2 } in
-    let h2 = ST.get () in
-    assert (as_ctx h2 res == S.bn_field_init (as_seq h0 n));
-    assert (S.bn_mont_ctx_inv (as_ctx h2 res));
-    B.(modifies_only_not_unused_in loc_none h0 h2);
-    res end
-  else begin
-    let mu = uint #t #SEC 0 in
-    let res : bn_mont_ctx t = { len = len; n = n1; mu = mu; r2 = r2 } in
-    let h2 = ST.get () in
-    B.(modifies_only_not_unused_in loc_none h0 h2);
-    res end
+  let mu = BM.mod_inv_limb n.(0ul) in
+  let res : bn_mont_ctx t = { len = len; n = n1; mu = mu; r2 = r2 } in
+  let h2 = ST.get () in
+  assert (as_ctx h2 res == S.bn_field_init (as_seq h0 n));
+  assert (S.bn_mont_ctx_inv (as_ctx h2 res));
+  B.(modifies_only_not_unused_in loc_none h0 h2);
+  B.malloc r res 1ul
 
 
 let bn_field_free #t k =
-  let n : buffer (limb t) = k.n in
-  let r2 : buffer (limb t) = k.r2 in
+  let open LowStar.BufferOps in
+  let k1 = !*k in
+  let n : buffer (limb t) = k1.n in
+  let r2 : buffer (limb t) = k1.r2 in
   B.free n;
   B.freeable_disjoint n r2;
-  B.free r2
+  B.free r2;
+  B.free k
 
 
 let bn_to_field #t km k a aM =
+  let open LowStar.BufferOps in
+  let k1 = !*k in
   let h0 = ST.get () in
-  km.BM.to k.n k.mu k.r2 a aM;
+  km.BM.to k1.n k1.mu k1.r2 a aM;
   let h1 = ST.get () in
-  assert (as_seq h1 aM == S.bn_to_field (as_ctx h0 k) (as_seq h0 a))
+  assert (as_seq h1 aM == S.bn_to_field (as_pctx h0 k) (as_seq h0 a))
 
 
 let bn_from_field #t km k aM a =
+  let open LowStar.BufferOps in
+  let k1 = !*k in
   let h0 = ST.get () in
-  km.BM.from k.n k.mu aM a;
+  km.BM.from k1.n k1.mu aM a;
   let h1 = ST.get () in
-  assert (as_seq h1 a == S.bn_from_field (as_ctx h0 k) (as_seq h0 aM))
+  assert (as_seq h1 a == S.bn_from_field (as_pctx h0 k) (as_seq h0 aM))
 
 
 let bn_field_add #t km k aM bM cM =
+  let open LowStar.BufferOps in
+  let k1 = !*k in
   let h0 = ST.get () in
-  km.BM.bn.BN.add_mod_n k.n aM bM cM;
+  km.BM.bn.BN.add_mod_n k1.n aM bM cM;
   let h1 = ST.get () in
-  assert (as_seq h1 cM == S.bn_field_add (as_ctx h0 k) (as_seq h0 aM) (as_seq h0 bM))
+  assert (as_seq h1 cM == S.bn_field_add (as_pctx h0 k) (as_seq h0 aM) (as_seq h0 bM))
 
 
 let bn_field_sub #t km k aM bM cM =
+  let open LowStar.BufferOps in
+  let k1 = !*k in
   let h0 = ST.get () in
-  BN.bn_sub_mod_n k.len k.n aM bM cM;
+  BN.bn_sub_mod_n k1.len k1.n aM bM cM;
   let h1 = ST.get () in
-  assert (as_seq h1 cM == S.bn_field_sub (as_ctx h0 k) (as_seq h0 aM) (as_seq h0 bM))
+  assert (as_seq h1 cM == S.bn_field_sub (as_pctx h0 k) (as_seq h0 aM) (as_seq h0 bM))
 
 
 let bn_field_mul #t km k aM bM cM =
+  let open LowStar.BufferOps in
+  let k1 = !*k in
   let h0 = ST.get () in
-  km.BM.mul k.n k.mu aM bM cM;
+  km.BM.mul k1.n k1.mu aM bM cM;
   let h1 = ST.get () in
-  assert (as_seq h1 cM == S.bn_field_mul (as_ctx h0 k) (as_seq h0 aM) (as_seq h0 bM))
+  assert (as_seq h1 cM == S.bn_field_mul (as_pctx h0 k) (as_seq h0 aM) (as_seq h0 bM))
 
 
 let bn_field_sqr #t km k aM cM =
+  let open LowStar.BufferOps in
+  let k1 = !*k in
   let h0 = ST.get () in
-  km.BM.sqr k.n k.mu aM cM;
+  km.BM.sqr k1.n k1.mu aM cM;
   let h1 = ST.get () in
-  assert (as_seq h1 cM == S.bn_field_sqr (as_ctx h0 k) (as_seq h0 aM))
+  assert (as_seq h1 cM == S.bn_field_sqr (as_pctx h0 k) (as_seq h0 aM))
 
 
 let bn_field_one #t km k oneM =
+  let open LowStar.BufferOps in
+  let k1 = !*k in
   let h0 = ST.get () in
-  BM.bn_mont_one km k.n k.mu k.r2 oneM;
+  BM.bn_mont_one km k1.n k1.mu k1.r2 oneM;
   let h1 = ST.get () in
-  assert (as_seq h1 oneM == S.bn_field_one (as_ctx h0 k))
+  assert (as_seq h1 oneM == S.bn_field_one (as_pctx h0 k))
 
 
 let bn_field_exp_consttime #t km k aM bBits b resM =
+  let open LowStar.BufferOps in
+  let k1 = !*k in
   push_frame ();
-  let aMc = create k.len (uint #t #SEC 0) in
+  let aMc = create k1.len (uint #t #SEC 0) in
   copy aMc aM;
-  ME.bn_exp_mont_consttime #t km k.n k.mu k.r2 aMc bBits b resM;
+  ME.bn_exp_mont_consttime #t km k1.n k1.mu k1.r2 aMc bBits b resM;
   let h0 = ST.get () in
-  assert (bn_v h0 aM < bn_v #t #k.len h0 k.n);
-  BD.bn_eval_inj (v k.len)
-    (S.bn_field_exp_consttime (as_ctx h0 k) (as_seq h0 aM) (v bBits) (as_seq h0 b))
+  assert (bn_v h0 aM < bn_v_n h0 k);
+  BD.bn_eval_inj (v k1.len)
+    (S.bn_field_exp_consttime (as_pctx h0 k) (as_seq h0 aM) (v bBits) (as_seq h0 b))
     (as_seq h0 resM);
   pop_frame ()
 
 
 let bn_field_exp_vartime #t km k aM bBits b resM =
+  let open LowStar.BufferOps in
+  let k1 = !*k in
   push_frame ();
-  let aMc = create k.len (uint #t #SEC 0) in
+  let aMc = create k1.len (uint #t #SEC 0) in
   copy aMc aM;
-  ME.bn_exp_mont_vartime #t km k.n k.mu k.r2 aMc bBits b resM;
+  ME.bn_exp_mont_vartime #t km k1.n k1.mu k1.r2 aMc bBits b resM;
   let h0 = ST.get () in
-  assert (bn_v h0 aM < bn_v #t #k.len h0 k.n);
-  BD.bn_eval_inj (v k.len)
-    (S.bn_field_exp_vartime (as_ctx h0 k) (as_seq h0 aM) (v bBits) (as_seq h0 b))
+  assert (bn_v h0 aM < bn_v_n h0 k);
+  BD.bn_eval_inj (v k1.len)
+    (S.bn_field_exp_vartime (as_pctx h0 k) (as_seq h0 aM) (v bBits) (as_seq h0 b))
     (as_seq h0 resM);
   pop_frame ()
 
 
-let bn_field_inv #t k bn_field_exp_vartime aM aInvM =
-  [@inline_let]
-  let len = k.len in
+let bn_field_inv #t len bn_field_exp_vartime k aM aInvM =
+  let open LowStar.BufferOps in
+  let k1 = !*k in
+  let len = k1.len in
   push_frame ();
   let n2 = create len (uint #t #SEC 0) in
-  BI.bn_mod_inv_prime_n2 len k.n n2;
-  bn_field_exp_vartime aM (k.len *! size (bits t)) n2 aInvM;
+  BI.bn_mod_inv_prime_n2 len k1.n n2;
+  bn_field_exp_vartime k aM (k1.len *! size (bits t)) n2 aInvM;
   pop_frame ()
