code/bignum/Hacl.Bignum.MontArithmetic.fsti
@@ -57,6 +57,11 @@ let bn_mont_ctx (t:limb_t) = bn_mont_ctx' t (lb t) (ll t)
 let bn_mont_ctx_u32 = bn_mont_ctx' U32 (lb U32) (ll U32)
 let bn_mont_ctx_u64 = bn_mont_ctx' U64 (lb U64) (ll U64)
 
+inline_for_extraction
+let pbn_mont_ctx (t:limb_t) = B.pointer (bn_mont_ctx t)
+
+let pbn_mont_ctx_u32 = B.pointer bn_mont_ctx_u32
+let pbn_mont_ctx_u64 = B.pointer bn_mont_ctx_u64
 
 inline_for_extraction noextract
 let as_ctx (#t:limb_t) (h:mem) (k:bn_mont_ctx t) : GTot (S.bn_mont_ctx t) = {
@@ -66,24 +71,62 @@ let as_ctx (#t:limb_t) (h:mem) (k:bn_mont_ctx t) : GTot (S.bn_mont_ctx t) = {
   S.r2 = as_seq h (k.r2 <: lbignum t k.len);
   }
 
-
 inline_for_extraction noextract
 let bn_mont_ctx_inv (#t:limb_t) (h:mem) (k:bn_mont_ctx t) =
-  live h (k.n <: lbignum t k.len) /\ live h (k.r2 <: lbignum t k.len) /\
-  disjoint (k.n <: lbignum t k.len) (k.r2 <: lbignum t k.len) /\
+  let n : buffer (limb t) = k.n in
+  let r2 : buffer (limb t) = k.r2 in
+  live h n /\ live h r2 /\ disjoint n r2 /\
   S.bn_mont_ctx_inv (as_ctx h k)
 
 
 inline_for_extraction noextract
-let bn_field_get_len_st (#t:limb_t) (k:bn_mont_ctx t) = unit ->
-  Stack (BN.meta_len t)
-  (requires fun h -> bn_mont_ctx_inv h k)
-  (ensures  fun h0 r h1 -> h0 == h1 /\
-    v r == S.bn_field_get_len (as_ctx h0 k))
+let bn_v_n (#t:limb_t) (h:mem) (k:pbn_mont_ctx t) =
+  let k1 = B.deref h k in
+  let n : lbignum t k1.len = k1.n in
+  bn_v h n
+
+inline_for_extraction noextract
+let freeable_s (#t:limb_t) (h:mem) (k:bn_mont_ctx t) =
+  let n : buffer (limb t) = k.n in
+  let r2 : buffer (limb t) = k.r2 in
+  B.freeable n /\ B.freeable r2
+
+inline_for_extraction noextract
+let freeable (#t:limb_t) (h:mem) (k:pbn_mont_ctx t) =
+  B.freeable k /\ freeable_s h (B.deref h k)
+
+inline_for_extraction noextract
+let footprint_s (#t:limb_t) (h:mem) (k:bn_mont_ctx t) =
+  let n : buffer (limb t) = k.n in
+  let r2 : buffer (limb t) = k.r2 in
+  B.(loc_union (loc_addr_of_buffer n) (loc_addr_of_buffer r2))
+
+inline_for_extraction noextract
+let footprint (#t:limb_t) (h:mem) (k:pbn_mont_ctx t) =
+  B.(loc_union (loc_addr_of_buffer k) (footprint_s h (B.deref h k)))
+
+inline_for_extraction noextract
+let as_pctx (#t:limb_t) (h:mem) (k:pbn_mont_ctx t) : GTot (S.bn_mont_ctx t) =
+  as_ctx h (B.deref h k)
+
+inline_for_extraction noextract
+let pbn_mont_ctx_inv (#t:limb_t) (h:mem) (k:pbn_mont_ctx t) =
+  B.live h k /\
+  B.(loc_disjoint (loc_addr_of_buffer k) (footprint_s h (B.deref h k))) /\
+  bn_mont_ctx_inv h (B.deref h k)
 
 
 inline_for_extraction noextract
-val bn_field_get_len: #t:limb_t -> k:bn_mont_ctx t -> bn_field_get_len_st k
+let bn_field_get_len_st (t:limb_t) = k:pbn_mont_ctx t ->
+  Stack (BN.meta_len t)
+  (requires fun h -> pbn_mont_ctx_inv h k)
+  (ensures  fun h0 r h1 -> h0 == h1 /\
+    r == (B.deref h0 k).len /\
+    v r == S.bn_field_get_len (as_pctx h0 k))
+
+
+inline_for_extraction noextract
+val bn_field_get_len: #t:limb_t -> bn_field_get_len_st t
 
 
 inline_for_extraction noextract
@@ -102,21 +145,18 @@ inline_for_extraction noextract
 let bn_field_init_st (t:limb_t) (len:BN.meta_len t) =
     r:HS.rid
   -> n:lbignum t len ->
-  ST (bn_mont_ctx t)
+  ST (pbn_mont_ctx t)
   (requires fun h ->
+    S.bn_mont_ctx_pre (as_seq h n) /\
+
     live h n /\ ST.is_eternal_region r)
   (ensures  fun h0 res h1 ->
     B.(modifies loc_none h0 h1) /\
-   (let n1 : buffer (limb t) = res.n in
-    let r2 : buffer (limb t) = res.r2 in
-    live h1 n1 /\ live h1 r2 /\ disjoint n1 r2 /\
-    B.(fresh_loc (loc_union (loc_buffer n1) (loc_buffer r2)) h0 h1) /\
-    B.(loc_includes (loc_region_only true r) (loc_union (loc_buffer n1) (loc_buffer r2))) /\
-    B.freeable n1 /\ B.freeable r2 /\
-
-   (S.bn_mont_ctx_pre (as_seq h0 n) ==> (
-      S.bn_mont_ctx_inv (as_ctx h1 res) /\
-      as_ctx h1 res == S.bn_field_init (as_seq h0 n)))))
+    B.(fresh_loc (footprint h1 res) h0 h1) /\
+    B.(loc_includes (loc_region_only true r) (footprint h1 res)) /\
+    freeable h1 res /\
+    S.bn_mont_ctx_inv (as_pctx h1 res) /\
+    as_pctx h1 res == S.bn_field_init (as_seq h0 n))
 
 
 inline_for_extraction noextract
@@ -124,17 +164,13 @@ val bn_field_init: #t:limb_t -> km:BM.mont t -> bn_field_init_st t km.BM.bn.BN.l
 
 
 inline_for_extraction noextract
-let bn_field_free_st (t:limb_t) = k:bn_mont_ctx t ->
+let bn_field_free_st (t:limb_t) = k:pbn_mont_ctx t ->
   ST unit
   (requires fun h ->
-   (let n : buffer (limb t) = k.n in
-    let r2 : buffer (limb t) = k.r2 in
-    live h n /\ live h r2 /\ disjoint n r2 /\
-    B.freeable n /\ B.freeable r2))
+    freeable h k /\
+    pbn_mont_ctx_inv h k)
   (ensures  fun h0 _ h1 ->
-    let n : buffer (limb t) = k.n in
-    let r2 : buffer (limb t) = k.r2 in
-    B.(modifies (loc_union (loc_addr_of_buffer r2) (loc_addr_of_buffer n)) h0 h1))
+    B.(modifies (footprint h0 k) h0 h1))
 
 
 inline_for_extraction noextract
@@ -142,245 +178,250 @@ val bn_field_free: #t:limb_t -> bn_field_free_st t
 
 
 inline_for_extraction noextract
-let bn_to_field_st (#t:limb_t) (k:bn_mont_ctx t) =
-    a:lbignum t k.len
-  -> aM:lbignum t k.len ->
+let bn_to_field_st (t:limb_t) (len:BN.meta_len t) =
+    k:pbn_mont_ctx t
+  -> a:lbignum t len
+  -> aM:lbignum t len ->
   Stack unit
   (requires fun h ->
-    bn_mont_ctx_inv h k /\
+    (B.deref h k).len == len /\
+    pbn_mont_ctx_inv h k /\
 
     live h a /\ live h aM /\ disjoint a aM /\
-    disjoint a (k.r2 <: lbignum t k.len) /\ disjoint a (k.n <: lbignum t k.len) /\
-    disjoint aM (k.r2 <: lbignum t k.len) /\ disjoint aM (k.n <: lbignum t k.len))
+    B.(loc_disjoint (footprint h k) (loc_buffer (a <: buffer (limb t)))) /\
+    B.(loc_disjoint (footprint h k) (loc_buffer (aM <: buffer (limb t)))))
   (ensures  fun h0 _ h1 -> modifies (loc aM) h0 h1 /\
-    bn_v h1 aM < bn_v #t #k.len h0 k.n /\
-    as_seq h1 aM == S.bn_to_field (as_ctx h0 k) (as_seq h0 a))
+    bn_v h1 aM < bn_v_n h0 k /\
+    as_seq h1 aM == S.bn_to_field (as_pctx h0 k) (as_seq h0 a))
 
 
 inline_for_extraction noextract
-val bn_to_field: #t:limb_t -> km:BM.mont t -> k:bn_mont_ctx t{k.len == km.BM.bn.BN.len} -> bn_to_field_st k
+val bn_to_field: #t:limb_t -> km:BM.mont t -> bn_to_field_st t km.BM.bn.BN.len
 
 
 inline_for_extraction noextract
-let bn_from_field_st (#t:limb_t) (k:bn_mont_ctx t) =
-    aM:lbignum t k.len
-  -> a:lbignum t k.len ->
+let bn_from_field_st (t:limb_t) (len:BN.meta_len t) =
+    k:pbn_mont_ctx t
+  -> aM:lbignum t len
+  -> a:lbignum t len ->
   Stack unit
   (requires fun h ->
-    bn_mont_ctx_inv h k /\ bn_v h aM < bn_v #t #k.len h k.n /\
+    (B.deref h k).len == len /\
+    pbn_mont_ctx_inv h k /\ bn_v h aM < bn_v_n h k /\
 
     live h a /\ live h aM /\ disjoint a aM /\
-    disjoint a (k.r2 <: lbignum t k.len) /\ disjoint a (k.n <: lbignum t k.len) /\
-    disjoint aM (k.r2 <: lbignum t k.len) /\ disjoint aM (k.n <: lbignum t k.len))
+    B.(loc_disjoint (footprint h k) (loc_buffer (a <: buffer (limb t)))) /\
+    B.(loc_disjoint (footprint h k) (loc_buffer (aM <: buffer (limb t)))))
   (ensures  fun h0 _ h1 -> modifies (loc a) h0 h1 /\
-    bn_v h1 a < bn_v #t #k.len h0 k.n /\
-    as_seq h1 a == S.bn_from_field (as_ctx h0 k) (as_seq h0 aM))
+    bn_v h1 a < bn_v_n h0 k /\
+    as_seq h1 a == S.bn_from_field (as_pctx h0 k) (as_seq h0 aM))
 
 
 inline_for_extraction noextract
-val bn_from_field: #t:limb_t -> km:BM.mont t -> k:bn_mont_ctx t{k.len == km.BM.bn.BN.len} -> bn_from_field_st k
+val bn_from_field: #t:limb_t -> km:BM.mont t -> bn_from_field_st t km.BM.bn.BN.len
 
 
 inline_for_extraction noextract
-let bn_field_add_st (#t:limb_t) (k:bn_mont_ctx t) =
-    aM:lbignum t k.len
-  -> bM:lbignum t k.len
-  -> cM:lbignum t k.len ->
+let bn_field_add_st (t:limb_t) (len:BN.meta_len t) =
+    k:pbn_mont_ctx t
+  -> aM:lbignum t len
+  -> bM:lbignum t len
+  -> cM:lbignum t len ->
   Stack unit
   (requires fun h ->
-    bn_mont_ctx_inv h k /\
-    bn_v h aM < bn_v #t #k.len h k.n /\
-    bn_v h bM < bn_v #t #k.len h k.n /\
+    (B.deref h k).len == len /\
+    pbn_mont_ctx_inv h k /\
+    bn_v h aM < bn_v_n h k /\
+    bn_v h bM < bn_v_n h k /\
 
     live h aM /\ live h bM /\ live h cM /\
     eq_or_disjoint aM bM /\ eq_or_disjoint aM cM /\ eq_or_disjoint bM cM /\
-    disjoint (k.n <: lbignum t k.len) aM /\
-    disjoint (k.n <: lbignum t k.len) bM /\
-    disjoint (k.n <: lbignum t k.len) cM)
+    B.(loc_disjoint (footprint h k) (loc_buffer (aM <: buffer (limb t)))) /\
+    B.(loc_disjoint (footprint h k) (loc_buffer (bM <: buffer (limb t)))) /\
+    B.(loc_disjoint (footprint h k) (loc_buffer (cM <: buffer (limb t)))))
   (ensures  fun h0 _ h1 -> modifies (loc cM) h0 h1 /\
-    bn_v h1 cM < bn_v #t #k.len h0 k.n /\
-    as_seq h1 cM == S.bn_field_add (as_ctx h0 k) (as_seq h0 aM) (as_seq h0 bM))
+    bn_v h1 cM < bn_v_n h0 k /\
+    as_seq h1 cM == S.bn_field_add (as_pctx h0 k) (as_seq h0 aM) (as_seq h0 bM))
 
 
 inline_for_extraction noextract
-val bn_field_add: #t:limb_t -> km:BM.mont t -> k:bn_mont_ctx t{k.len == km.BM.bn.BN.len} -> bn_field_add_st k
+val bn_field_add: #t:limb_t -> km:BM.mont t -> bn_field_add_st t km.BM.bn.BN.len
 
 
 inline_for_extraction noextract
-let bn_field_sub_st (#t:limb_t) (k:bn_mont_ctx t) =
-    aM:lbignum t k.len
-  -> bM:lbignum t k.len
-  -> cM:lbignum t k.len ->
+let bn_field_sub_st (t:limb_t) (len:BN.meta_len t) =
+    k:pbn_mont_ctx t
+  -> aM:lbignum t len
+  -> bM:lbignum t len
+  -> cM:lbignum t len ->
   Stack unit
   (requires fun h ->
-    bn_mont_ctx_inv h k /\
-    bn_v h aM < bn_v #t #k.len h k.n /\
-    bn_v h bM < bn_v #t #k.len h k.n /\
+    (B.deref h k).len == len /\
+    pbn_mont_ctx_inv h k /\
+    bn_v h aM < bn_v_n h k /\
+    bn_v h bM < bn_v_n h k /\
 
     live h aM /\ live h bM /\ live h cM /\
     eq_or_disjoint aM bM /\ eq_or_disjoint aM cM /\ eq_or_disjoint bM cM /\
-    disjoint (k.n <: lbignum t k.len) aM /\
-    disjoint (k.n <: lbignum t k.len) bM /\
-    disjoint (k.n <: lbignum t k.len) cM)
+    B.(loc_disjoint (footprint h k) (loc_buffer (aM <: buffer (limb t)))) /\
+    B.(loc_disjoint (footprint h k) (loc_buffer (bM <: buffer (limb t)))) /\
+    B.(loc_disjoint (footprint h k) (loc_buffer (cM <: buffer (limb t)))))
   (ensures  fun h0 _ h1 -> modifies (loc cM) h0 h1 /\
-    bn_v h1 cM < bn_v #t #k.len h0 k.n /\
-    as_seq h1 cM == S.bn_field_sub (as_ctx h0 k) (as_seq h0 aM) (as_seq h0 bM))
+    bn_v h1 cM < bn_v_n h0 k /\
+    as_seq h1 cM == S.bn_field_sub (as_pctx h0 k) (as_seq h0 aM) (as_seq h0 bM))
 
 
 inline_for_extraction noextract
-val bn_field_sub: #t:limb_t -> km:BM.mont t -> k:bn_mont_ctx t{k.len == km.BM.bn.BN.len} -> bn_field_sub_st k
+val bn_field_sub: #t:limb_t -> km:BM.mont t -> bn_field_sub_st t km.BM.bn.BN.len
 
 
 inline_for_extraction noextract
-let bn_field_mul_st (#t:limb_t) (k:bn_mont_ctx t) =
-    aM:lbignum t k.len
-  -> bM:lbignum t k.len
-  -> cM:lbignum t k.len ->
+let bn_field_mul_st (t:limb_t) (len:BN.meta_len t) =
+    k:pbn_mont_ctx t
+  -> aM:lbignum t len
+  -> bM:lbignum t len
+  -> cM:lbignum t len ->
   Stack unit
   (requires fun h ->
-    bn_mont_ctx_inv h k /\
-    bn_v h aM < bn_v #t #k.len h k.n /\
-    bn_v h bM < bn_v #t #k.len h k.n /\
+    (B.deref h k).len == len /\
+    pbn_mont_ctx_inv h k /\
+    bn_v h aM < bn_v_n h k /\
+    bn_v h bM < bn_v_n h k /\
 
     live h aM /\ live h bM /\ live h cM /\
     eq_or_disjoint aM bM /\ eq_or_disjoint aM cM /\ eq_or_disjoint bM cM /\
-    disjoint cM (k.n <: lbignum t k.len))
+    B.(loc_disjoint (footprint h k) (loc_buffer (aM <: buffer (limb t)))) /\
+    B.(loc_disjoint (footprint h k) (loc_buffer (bM <: buffer (limb t)))) /\
+    B.(loc_disjoint (footprint h k) (loc_buffer (cM <: buffer (limb t)))))
   (ensures  fun h0 _ h1 -> modifies (loc cM) h0 h1 /\
-    bn_v h1 cM < bn_v #t #k.len h0 k.n /\
-    as_seq h1 cM == S.bn_field_mul (as_ctx h0 k) (as_seq h0 aM) (as_seq h0 bM))
+    bn_v h1 cM < bn_v_n h0 k /\
+    as_seq h1 cM == S.bn_field_mul (as_pctx h0 k) (as_seq h0 aM) (as_seq h0 bM))
 
 
 inline_for_extraction noextract
-val bn_field_mul: #t:limb_t -> km:BM.mont t -> k:bn_mont_ctx t{k.len == km.BM.bn.BN.len} -> bn_field_mul_st k
+val bn_field_mul: #t:limb_t -> km:BM.mont t -> bn_field_mul_st t km.BM.bn.BN.len
 
 
 inline_for_extraction noextract
-let bn_field_sqr_st (#t:limb_t) (k:bn_mont_ctx t) =
-    aM:lbignum t k.len
-  -> cM:lbignum t k.len ->
+let bn_field_sqr_st (t:limb_t) (len:BN.meta_len t) =
+    k:pbn_mont_ctx t
+  -> aM:lbignum t len
+  -> cM:lbignum t len ->
   Stack unit
   (requires fun h ->
-    bn_mont_ctx_inv h k /\
-    bn_v h aM < bn_v #t #k.len h k.n /\
+    (B.deref h k).len == len /\
+    pbn_mont_ctx_inv h k /\
+    bn_v h aM < bn_v_n h k /\
 
-    live h aM /\ live h cM /\
-    eq_or_disjoint aM cM /\ disjoint cM (k.n <: lbignum t k.len))
+    live h aM /\ live h cM /\ eq_or_disjoint aM cM /\
+    B.(loc_disjoint (footprint h k) (loc_buffer (aM <: buffer (limb t)))) /\
+    B.(loc_disjoint (footprint h k) (loc_buffer (cM <: buffer (limb t)))))
   (ensures  fun h0 _ h1 -> modifies (loc cM) h0 h1 /\
-    bn_v h1 cM < bn_v #t #k.len h0 k.n /\
-    as_seq h1 cM == S.bn_field_sqr (as_ctx h0 k) (as_seq h0 aM))
+    bn_v h1 cM < bn_v_n h0 k /\
+    as_seq h1 cM == S.bn_field_sqr (as_pctx h0 k) (as_seq h0 aM))
 
 
 inline_for_extraction noextract
-val bn_field_sqr: #t:limb_t -> km:BM.mont t -> k:bn_mont_ctx t{k.len == km.BM.bn.BN.len} -> bn_field_sqr_st k
+val bn_field_sqr: #t:limb_t -> km:BM.mont t -> bn_field_sqr_st t km.BM.bn.BN.len
 
 
 inline_for_extraction noextract
-let bn_field_one_st (#t:limb_t) (k:bn_mont_ctx t) = oneM:lbignum t k.len ->
+let bn_field_one_st (t:limb_t) (len:BN.meta_len t) =
+    k:pbn_mont_ctx t
+  -> oneM:lbignum t len ->
   Stack unit
   (requires fun h ->
-    bn_mont_ctx_inv h k /\
+    (B.deref h k).len == len /\
+    pbn_mont_ctx_inv h k /\
 
     live h oneM /\
-    disjoint (k.n <: lbignum t k.len) oneM /\
-    disjoint (k.r2 <: lbignum t k.len) oneM)
+    B.(loc_disjoint (footprint h k) (loc_buffer (oneM <: buffer (limb t)))))
   (ensures  fun h0 _ h1 -> modifies (loc oneM) h0 h1 /\
-    bn_v h1 oneM < bn_v #t #k.len h0 k.n /\
-    as_seq h1 oneM == S.bn_field_one (as_ctx h0 k))
+    bn_v h1 oneM < bn_v_n h0 k /\
+    as_seq h1 oneM == S.bn_field_one (as_pctx h0 k))
 
 
 inline_for_extraction noextract
-val bn_field_one: #t:limb_t -> km:BM.mont t -> k:bn_mont_ctx t{k.len == km.BM.bn.BN.len} -> bn_field_one_st k
+val bn_field_one: #t:limb_t -> km:BM.mont t -> bn_field_one_st t km.BM.bn.BN.len
 
 
 inline_for_extraction noextract
-let bn_field_exp_consttime_st (#t:limb_t) (k:bn_mont_ctx t) =
-    aM:lbignum t k.len
+let bn_field_exp_consttime_st (t:limb_t) (len:BN.meta_len t) =
+    k:pbn_mont_ctx t
+  -> aM:lbignum t len
   -> bBits:size_t{0 < v bBits}
   -> b:lbignum t (blocks bBits (size (bits t)))
-  -> resM:lbignum t k.len ->
+  -> resM:lbignum t len ->
   Stack unit
   (requires fun h ->
-    bn_mont_ctx_inv h k /\
-    bn_v h aM < bn_v #t #k.len h k.n /\
+    (B.deref h k).len == len /\
+    pbn_mont_ctx_inv h k /\
+    bn_v h aM < bn_v_n h k /\
     0 < bn_v h b /\ bn_v h b < pow2 (v bBits) /\
 
     live h aM /\ live h b /\ live h resM /\
-    disjoint resM aM /\ disjoint resM b /\
-    disjoint aM b /\
-    disjoint (k.n <: lbignum t k.len) resM /\
-    disjoint (k.n <: lbignum t k.len) aM /\
-    disjoint (k.r2 <: lbignum t k.len) resM /\
-    disjoint (k.r2 <: lbignum t k.len) aM)
+    disjoint resM aM /\ disjoint resM b /\ disjoint aM b /\
+    B.(loc_disjoint (footprint h k) (loc_buffer (aM <: buffer (limb t)))) /\
+    B.(loc_disjoint (footprint h k) (loc_buffer (resM <: buffer (limb t)))))
   (ensures  fun h0 _ h1 -> modifies (loc resM) h0 h1 /\
-    bn_v h1 resM < bn_v #t #k.len h0 k.n /\
-    as_seq h1 resM == S.bn_field_exp_consttime (as_ctx h0 k) (as_seq h0 aM) (v bBits) (as_seq h0 b))
+    bn_v h1 resM < bn_v_n h0 k /\
+    as_seq h1 resM == S.bn_field_exp_consttime (as_pctx h0 k) (as_seq h0 aM) (v bBits) (as_seq h0 b))
 
 
 inline_for_extraction noextract
-val bn_field_exp_consttime:
-    #t:limb_t
-  -> km:BM.mont t
-  -> k:bn_mont_ctx t{k.len == km.BM.bn.BN.len} ->
-  bn_field_exp_consttime_st k
+val bn_field_exp_consttime: #t:limb_t -> km:BM.mont t -> bn_field_exp_consttime_st t km.BM.bn.BN.len
 
 
 inline_for_extraction noextract
-let bn_field_exp_vartime_st (#t:limb_t) (k:bn_mont_ctx t) =
-    aM:lbignum t k.len
+let bn_field_exp_vartime_st (t:limb_t) (len:BN.meta_len t) =
+    k:pbn_mont_ctx t
+  -> aM:lbignum t len
   -> bBits:size_t{0 < v bBits}
   -> b:lbignum t (blocks bBits (size (bits t)))
-  -> resM:lbignum t k.len ->
+  -> resM:lbignum t len ->
   Stack unit
   (requires fun h ->
-    bn_mont_ctx_inv h k /\
-    bn_v h aM < bn_v #t #k.len h k.n /\
+    (B.deref h k).len == len /\
+    pbn_mont_ctx_inv h k /\
+    bn_v h aM < bn_v_n h k /\
     0 < bn_v h b /\ bn_v h b < pow2 (v bBits) /\
 
     live h aM /\ live h b /\ live h resM /\
-    disjoint resM aM /\ disjoint resM b /\
-    disjoint aM b /\
-    disjoint (k.n <: lbignum t k.len) resM /\
-    disjoint (k.n <: lbignum t k.len) aM /\
-    disjoint (k.r2 <: lbignum t k.len) resM /\
-    disjoint (k.r2 <: lbignum t k.len) aM)
+    disjoint resM aM /\ disjoint resM b /\ disjoint aM b /\
+    B.(loc_disjoint (footprint h k) (loc_buffer (aM <: buffer (limb t)))) /\
+    B.(loc_disjoint (footprint h k) (loc_buffer (resM <: buffer (limb t)))))
   (ensures  fun h0 _ h1 -> modifies (loc resM) h0 h1 /\
-    bn_v h1 resM < bn_v #t #k.len h0 k.n /\
-    as_seq h1 resM == S.bn_field_exp_vartime (as_ctx h0 k) (as_seq h0 aM) (v bBits) (as_seq h0 b))
+    bn_v h1 resM < bn_v_n h0 k /\
+    as_seq h1 resM == S.bn_field_exp_vartime (as_pctx h0 k) (as_seq h0 aM) (v bBits) (as_seq h0 b))
 
 
 inline_for_extraction noextract
-val bn_field_exp_vartime:
-    #t:limb_t
-  -> km:BM.mont t
-  -> k:bn_mont_ctx t{k.len == km.BM.bn.BN.len} ->
-  bn_field_exp_vartime_st k
-
+val bn_field_exp_vartime: #t:limb_t -> km:BM.mont t -> bn_field_exp_vartime_st t km.BM.bn.BN.len
 
 
 inline_for_extraction noextract
-let bn_field_inv_st (#t:limb_t) (k:bn_mont_ctx t) =
-    aM:lbignum t k.len
-  -> aInvM:lbignum t k.len ->
+let bn_field_inv_st (t:limb_t) (len:BN.meta_len t) =
+    k:pbn_mont_ctx t
+  -> aM:lbignum t len
+  -> aInvM:lbignum t len ->
   Stack unit
   (requires fun h ->
-    bn_mont_ctx_inv h k /\
-    Euclid.is_prime (bn_v #t #k.len h k.n) /\
-    0 < bn_v h aM /\ bn_v h aM < bn_v #t #k.len h k.n /\
+    (B.deref h k).len == len /\
+    pbn_mont_ctx_inv h k /\
+    Euclid.is_prime (bn_v_n h k) /\
+    0 < bn_v h aM /\ bn_v h aM < bn_v_n h k /\
 
-    live h aM /\ live h aInvM /\
-    disjoint aM aInvM /\
-    disjoint (k.n <: lbignum t k.len) aM /\
-    disjoint (k.n <: lbignum t k.len) aInvM /\
-    disjoint (k.r2 <: lbignum t k.len) aM /\
-    disjoint (k.r2 <: lbignum t k.len) aInvM)
+    live h aM /\ live h aInvM /\ disjoint aM aInvM /\
+    B.(loc_disjoint (footprint h k) (loc_buffer (aM <: buffer (limb t)))) /\
+    B.(loc_disjoint (footprint h k) (loc_buffer (aInvM <: buffer (limb t)))))
   (ensures  fun h0 _ h1 -> modifies (loc aInvM) h0 h1 /\
-    bn_v h1 aInvM < bn_v #t #k.len h0 k.n /\
-    as_seq h1 aInvM == S.bn_field_inv (as_ctx h0 k) (as_seq h0 aM))
+    bn_v h1 aInvM < bn_v_n h0 k /\
+    as_seq h1 aInvM == S.bn_field_inv (as_pctx h0 k) (as_seq h0 aM))
 
 
 inline_for_extraction noextract
 val bn_field_inv:
     #t:limb_t
-  -> k:bn_mont_ctx t
-  -> bn_field_exp_vartime:bn_field_exp_vartime_st k ->
-  bn_field_inv_st k
+  -> len:Ghost.erased _
+  -> bn_field_exp_vartime:bn_field_exp_vartime_st t len ->
+  bn_field_inv_st t len
